fix in computation of transition relation fixes in specs

Test/civl/inductive-sequentialization/paxos/PaxosAbstractions.bpl
@@ -23,150 +23,56 @@ procedure {:IS_abstraction}{:layer 2} A_StartRound'(r: Round, {:linear_in "perm"
 returns ({:pending_async "A_Join", "A_Propose"} PAs:[PA]int)
 modifies pendingAsyncs;
 {
-  assert r == r_lin;
-  assert Round(r);
-  assert pendingAsyncs[A_StartRound(r, r_lin)] > 0;
-
-  /**************************************************************************/
-  // Hint for left mover checks
   assert
     {:add_to_pool "Round", r-1}
     {:add_to_pool "Node", 0}
     RoundCollector(r)[ConcludePerm(r)];
-  /**************************************************************************/
-
-  PAs := MapAdd(JoinPAs(r), SingletonPA(A_Propose(r, ProposePermissions(r))));
-
-  pendingAsyncs := MapAdd(pendingAsyncs, PAs);
-  pendingAsyncs := MapSub(pendingAsyncs, SingletonPA(A_StartRound(r, r_lin)));
+  call PAs := A_StartRound(r, r_lin);
 }
 
 procedure {:IS_abstraction}{:layer 2} A_Propose'(r: Round, {:linear_in "perm"} ps: [Permission]bool)
 returns ({:pending_async "A_Vote", "A_Conclude"} PAs:[PA]int)
 modifies voteInfo, pendingAsyncs;
 {
-  var {:pool "Round"} maxRound: int;
-  var maxValue: Value;
-  var {:pool "NodeSet"} ns: NodeSet;
-
-  assert Round(r);
-  assert pendingAsyncs[A_Propose(r, ps)] > 0;
-  assert ps == ProposePermissions(r);
-  assert is#None(voteInfo[r]);
-
-  /**************************************************************************/
   assert (forall r': Round :: r' <= r ==> pendingAsyncs[A_StartRound(r', r')] == 0);
   assert (forall r': Round, n': Node, p': Permission :: r' <= r ==> pendingAsyncs[A_Join(r', n', p')] == 0);
   assert (forall r': Round, p': [Permission]bool :: r' < r ==> pendingAsyncs[A_Propose(r', p')] == 0);
-  assert (forall r': Round, n': Node, v': Value, p': Permission :: r' <= r ==> pendingAsyncs[A_Vote(r', n', v', p')] == 0);
-
-  // Hint for commutativity w.r.t. {Paxos, Propose}
+  assert (forall r': Round, n': Node, v': Value, p': Permission :: r' < r ==> pendingAsyncs[A_Vote(r', n', v', p')] == 0);
+  assert (forall r': Round, v': Value, p': Permission :: r' < r ==> pendingAsyncs[A_Conclude(r', v', p')] == 0);
   assert
     {:add_to_pool "Round", r, r-1}
     {:add_to_pool "Node", 0}
     ps[ConcludePerm(r)];
-  /**************************************************************************/
-
-  assume
-    {:add_to_pool "NodeSet", ns}
-    true;
-
-  if (*) {
-    assume IsSubset(ns, joinedNodes[r]) && IsQuorum(ns);
-    maxRound := MaxRound(r, ns, voteInfo);
-    if (maxRound != 0)
-    {
-      maxValue := value#VoteInfo(t#Some(voteInfo[maxRound]));
-    }
-    voteInfo[r] := Some(VoteInfo(maxValue, NoNodes()));
-    PAs := MapAdd(VotePAs(r, maxValue), SingletonPA(A_Conclude(r, maxValue, ConcludePerm(r))));
-  } else {
-    PAs := NoPAs();
-  }
-
-  pendingAsyncs := MapAdd(pendingAsyncs, PAs);
-  pendingAsyncs := MapSub(pendingAsyncs, SingletonPA(A_Propose(r, ps)));
+  call PAs := A_Propose(r, ps);
 }
 
 procedure {:IS_abstraction}{:layer 2} A_Conclude'(r: Round, v: Value, {:linear_in "perm"} p: Permission)
 modifies decision, pendingAsyncs;
 {
-  var q: NodeSet;
-
-  assert Round(r);
-  assert pendingAsyncs[A_Conclude(r, v, p)] > 0;
-  assert p == ConcludePerm(r);
-  assert is#Some(voteInfo[r]);
-  assert value#VoteInfo(t#Some(voteInfo[r])) == v;
-
-  /**************************************************************************/
   assert
     {:add_to_pool "Round", r}
     (forall n': Node, v': Value, p': Permission :: pendingAsyncs[A_Vote(r, n', v', p')] == 0);
-  /**************************************************************************/
-
-  if (*) {
-    assume IsSubset(q, ns#VoteInfo(t#Some(voteInfo[r]))) && IsQuorum(q);
-    decision[r] := Some(v);
-  }
-
-  pendingAsyncs := MapSub(pendingAsyncs, SingletonPA(A_Conclude(r, v, p)));
+  call A_Conclude(r, v, p);
 }
 
 procedure {:IS_abstraction}{:layer 2} A_Join'(r: Round, n: Node, {:linear_in "perm"} p: Permission)
 modifies joinedNodes, pendingAsyncs;
 {
-  assert Round(r);
-  assert pendingAsyncs[A_Join(r, n, p)] > 0;
-  assert p == JoinPerm(r, n);
-
-  /**************************************************************************/
   assert (forall r': Round :: r' <= r ==> pendingAsyncs[A_StartRound(r', r')] == 0);
   assert (forall r': Round, n': Node, p': Permission :: r' < r ==> pendingAsyncs[A_Join(r', n', p')] == 0);
   assert (forall r': Round, p': [Permission]bool :: r' < r ==> pendingAsyncs[A_Propose(r', p')] == 0);
   assert (forall r': Round, n': Node, v': Value, p': Permission :: r' < r ==> pendingAsyncs[A_Vote(r', n', v', p')] == 0);
-  /**************************************************************************/
-
-  assume
-    {:add_to_pool "Round", r, r-1}
-    {:add_to_pool "Node", n}
-    true;
-  if (*) {
-    assume (forall r': Round :: Round(r') && joinedNodes[r'][n] ==> r' < r);
-    joinedNodes[r][n] := true;
-  }
-
-  pendingAsyncs := MapSub(pendingAsyncs, SingletonPA(A_Join(r, n, p)));
+  call A_Join(r, n, p);
 }
 
 procedure {:IS_abstraction}{:layer 2} A_Vote'(r: Round, n: Node, v: Value, {:linear_in "perm"} p: Permission)
 modifies joinedNodes, voteInfo, pendingAsyncs;
 {
-  assert Round(r);
-  assert p == VotePerm(r, n);
-  assert pendingAsyncs[A_Vote(r, n, v, p)] > 0;
-  assert is#Some(voteInfo[r]);
-  assert value#VoteInfo(t#Some(voteInfo[r])) == v;
-  assert !ns#VoteInfo(t#Some(voteInfo[r]))[n];
-
-  /**************************************************************************/
   assert (forall r': Round :: r' <= r ==> pendingAsyncs[A_StartRound(r', r')] == 0);
   assert (forall r': Round, n': Node, p': Permission :: r' <= r ==> pendingAsyncs[A_Join(r', n', p')] == 0);
   assert (forall r': Round, p': [Permission]bool :: r' <= r ==> pendingAsyncs[A_Propose(r', p')] == 0);
   assert (forall r': Round, n': Node, v': Value, p': Permission :: r' < r ==> pendingAsyncs[A_Vote(r', n', v', p')] == 0);
-  /**************************************************************************/
-
-  assume
-    {:add_to_pool "Round", r, r-1}
-    {:add_to_pool "Node", n}
-    true;
-  if (*) {
-    assume (forall r': Round :: Round(r') && joinedNodes[r'][n] ==> r' <= r);
-    voteInfo[r] := Some(VoteInfo(v, ns#VoteInfo(t#Some(voteInfo[r]))[n := true]));
-    joinedNodes[r][n] := true;
-  }
-
-  pendingAsyncs := MapSub(pendingAsyncs, SingletonPA(A_Vote(r, n, v, p)));
+  call A_Vote(r, n, v, p);
 }
 
 // Local Variables:
